coq: ZF: Meta: remove Signature

coq/ZF/Meta/Sigs.v
@@ -1,9 +1,0 @@
-Require Import Coq.Lists.List.
-Require Import Coq.Strings.String.
-
-Require Import ZF.Meta.Ty.
-Require Import ZF.Meta.Signature.
-
-Definition Sigs : Type := string -> option Signature.
-
-Definition empty : Sigs := fun _ => None.
