coq/ZF/Meta/Signature.v
@@ -1,5 +1,0 @@
-Require Import Coq.Lists.List.
-
-Require Import ZF.Meta.Ty.
-
-Definition Signature : Type := list Ty * Ty.
