coq/ZF/Meta/Test/Decl/Class/Incl.v
@@ -53,8 +53,8 @@ Proposition InclCheckIdent : forall (e:Env) (G:Ctx) (m n:nat),
 Proof.
   (* Proof by Hermes + gpt 5.5                                                  *)
   intros e G m n H1 H2 H3.
-  apply HasTyIdentT with [TyClass; TyClass].
-  - unfold Env.toSigs. rewrite H1. reflexivity.
+  apply HasTyIdentT with (d:=Incl).
+  - assumption.
   - apply HasTyTsCons.
     + apply HasTyVar. assumption.
     + apply HasTyTsCons.
